Wrapper

src/TicketLock.v
@@ -1,65 +1,44 @@
 From sflib Require Import sflib.
 From Paco Require Import paco.
 Require Import Coq.Classes.RelationClasses Lia Program.
-From Fairness Require Export ITreeLib WFLib FairBeh NatStructs Mod pind.
+From Fairness Require Export ITreeLib WFLib FairBeh NatStructs Mod pind Axioms OpenMod SCM Red IRed Wrapper.
+From Ordinal Require Export ClassicalHessenberg.
+
 
 Set Implicit Arguments.
 
 
 Module FairLock.
-  Definition all_fail (s: TIdSet.t): fmap thread_id :=
-    fun id => if (NatMap.mem id s) then Flag.fail else Flag.emp.
+  Definition lock_fun: WMod.function (option thread_id) unit void :=
+    WMod.mk_fun
+      tt
+      (fun tid (_: unit) st next =>
+         match st with
+         | None => next = WMod.normal (Some tid) tt (sum_fmap_l (fun _ => Flag.fail))
+         | Some _ => next = WMod.disabled
+         end).
 
-  Definition all_success (s: TIdSet.t): fmap thread_id :=
-    fun id => if (NatMap.mem id s) then Flag.success else Flag.emp.
+  Definition unlock_fun: WMod.function (option thread_id) unit void :=
+    WMod.mk_fun
+      tt
+      (fun tid (_: unit) st next =>
+         match st with
+         | None => next = WMod.stuck
+         | Some tid' =>
+             if (tid_dec tid' tid) then next = WMod.stuck
+             else next = WMod.normal None tt (sum_fmap_l (fun _ => Flag.emp))
+         end).
 
-  Definition lock_fun:
-    ktree (((@eventE thread_id) +' cE) +' sE (TIdSet.t * option thread_id)) unit unit :=
-    fun _ =>
-      _ <- trigger Yield;;
-      tid <- trigger GetTid;;
-      '(W, own) <- trigger (@Get _);;
-      let W := TIdSet.add tid W in
-      _ <- trigger (Put (W, own));;
+  Definition wmod: WMod.t :=
+    WMod.mk
+      None
+      [("lock", lock_fun);
+       ("unlock", unlock_fun)
+      ].
 
-      _ <- ITree.iter
-             (fun (_: unit) =>
-                '(W, own) <- trigger (@Get _);;
-                match own with
-                | Some _ => _ <- trigger Yield;; Ret (inl tt)
-                | None => Ret (inr tt)
-                end
-             ) tt;;
-
-      let W := TIdSet.remove tid W in
-      _ <- trigger (Fair (all_fail W));;
-      _ <- trigger (Put (W, Some tid));;
-      trigger Yield
-  .
-
-  Definition unlock_fun:
-    ktree (((@eventE thread_id) +' cE) +' sE (TIdSet.t * option thread_id)) unit unit :=
-    fun _ =>
-      _ <- trigger Yield;;
-      tid <- trigger GetTid;;
-      '(W, own) <- trigger (@Get _);;
-      own <- unwrap own;;
-      if (PeanoNat.Nat.eq_dec own tid)
-      then
-        _ <- trigger (Put (W, None));;
-        trigger Yield
-      else UB
-  .
-
-  Definition example_mod_spec: Mod.t :=
-    Mod.mk
-      (TIdSet.empty, None)
-      (Mod.get_funs [("lock", Mod.wrap_fun lock_fun);
-                     ("unlock", Mod.wrap_fun unlock_fun)
-      ]).
+  Definition mod: Mod.t :=
+    WMod.interp_mod wmod.
 End FairLock.
-
-From Fairness Require Import OpenMod SCM.
 
 Module TicketLock.
   Definition now_serving: SCMem.val := SCMem.val_ptr (0, 0).
@@ -68,19 +47,11 @@ Module TicketLock.
   Definition lock_fun:
     ktree ((((@eventE void) +' cE) +' (sE unit)) +' OpenMod.callE) unit unit :=
     fun _ =>
-      _ <- trigger Yield;;
-      myticket <- trigger (OpenMod.Call "faa" (next_ticket, 1)↑);;
-      myticket <- unwrap (myticket↓);;
-      _ <- trigger Yield;;
-
+      myticket <- (OMod.call "faa" (next_ticket, 1));;
       _ <- ITree.iter
              (fun (_: unit) =>
-                _ <- trigger Yield;;
-                next <- trigger (OpenMod.Call "load" (now_serving)↑);; next <- unwrap (next↓);;
-                _ <- trigger Yield;;
-                b <- trigger (OpenMod.Call "compare" (next: SCMem.val, myticket: SCMem.val)↑);; b <- unwrap (b↓);;
-                _ <- trigger Yield;;
-                if (b: bool) then Ret (inr tt) else Ret (inl tt)) tt;;
+                next <- (OMod.call "load" (now_serving));;
+                b <- (OMod.call "compare" (next: SCMem.val, myticket: SCMem.val));;          if (b: bool) then Ret (inr tt) else Ret (inl tt)) tt;;
       trigger Yield
   .
 
@@ -88,7 +59,308 @@ Module TicketLock.
     ktree ((((@eventE void) +' cE) +' (sE unit)) +' OpenMod.callE) unit unit :=
     fun _ =>
       _ <- trigger Yield;;
-      _ <- trigger (OpenMod.Call "faa" (now_serving, 1)↑);;
+      `_: unit <- (OMod.call "faa" (now_serving, 1));;
       trigger Yield
   .
+
+  Definition omod: OMod.t :=
+    OMod.mk
+      tt
+      (Mod.get_funs [("lock", Mod.wrap_fun lock_fun);
+                     ("unlock", Mod.wrap_fun unlock_fun)])
+  .
+
+  Definition mod: Mod.t :=
+    OMod.close
+      (omod)
+      (SCMem.mod [1; 1])
+  .
 End TicketLock.
+
+From Fairness Require Import IProp IPM Weakest.
+From Fairness Require Import ModSim PCM MonotonePCM ThreadsRA StateRA FairRA.
+
+
+
+Section SIM.
+  Context `{Σ: GRA.t}.
+  Context `{EXCL: @GRA.inG (Excl.t unit) Σ}.
+  Context `{MONORA: @GRA.inG monoRA Σ}.
+  Context `{THSRA: @GRA.inG ths_RA Σ}.
+  Context `{STATESRC: @GRA.inG (stateSrcRA unit) Σ}.
+  Context `{STATETGT: @GRA.inG (stateTgtRA (unit * SCMem.t)) Σ}.
+  Context `{IDENTSRC: @GRA.inG (identSrcRA void nat_wf) Σ}.
+  Context `{IDENTTGT: @GRA.inG (identTgtRA (void + SCMem.pointer)%type) Σ}.
+  Context `{IDENTTHS: @GRA.inG identThsRA Σ}.
+  Context `{MEMRA: @GRA.inG memRA Σ}.
+
+  Global Program Instance ge_PreOrder: PreOrder ge.
+  Next Obligation.
+  Proof.
+    ii. lia.
+  Qed.
+  Next Obligation.
+  Proof.
+    ii. lia.
+  Qed.
+
+
+  Definition partial_map_le A B (f0 f1: A -> option B): Prop :=
+    forall a b (SOME: f0 a = Some b), f1 a = Some b.
+
+  Global Program Instance partial_map_PreOrder A B: PreOrder (@partial_map_le A B).
+  Next Obligation.
+  Proof.
+    ii. auto.
+  Qed.
+  Next Obligation.
+  Proof.
+    ii. eapply H0. eapply H. auto.
+  Qed.
+
+  Definition partial_map_empty A B: A -> option B :=
+    fun _ => None.
+
+  Definition partial_map_update A B (a: A) (b: B) (f: A -> option B):
+    A -> option B :=
+    fun a' => if (excluded_middle_informative (a' = a)) then Some b else (f a').
+
+  Definition partial_map_singleton A B (a: A) (b: B): A -> option B :=
+    partial_map_update a b (@partial_map_empty A B).
+
+  Definition partial_map_update_le A B (a: A) (b: B) (f: A -> option B)
+             (NONE: f a = None)
+    :
+    partial_map_le f (partial_map_update a b f).
+  Proof.
+    ii. unfold partial_map_update. des_ifs.
+  Qed.
+
+  Definition partial_map_update_le_singleton A B (a: A) (b: B) (f: A -> option B)
+             (NONE: f a = None)
+    :
+    partial_map_le (partial_map_singleton a b) (partial_map_update a b f).
+  Proof.
+    ii. unfold partial_map_singleton, partial_map_update in *. des_ifs.
+  Qed.
+
+  Lemma partial_map_singleton_le_iff A B (a: A) (b: B) f
+    :
+    partial_map_le (partial_map_singleton a b) f <-> (f a = Some b).
+  Proof.
+    split.
+    { i. eapply H. unfold partial_map_singleton, partial_map_update. des_ifs. }
+    { ii. unfold partial_map_singleton, partial_map_update in *. des_ifs. }
+  Qed.
+
+  Fixpoint waiters now_serving (n: nat): iProp :=
+    match n with
+    | 0 => True
+    | S n => (∃ i, (monoWhite 1 (@partial_map_PreOrder nat nat) (partial_map_singleton (now_serving + n) i)) ** Pending i) ** (waiters now_serving n)
+    end.
+
+  Let I: iProp :=
+        (∃ m,
+            (memory_black m)
+              **
+              (St_tgt (tt, m)))
+          **
+          (∃ now_serving n f i,
+              (points_to TicketLock.next_ticket (SCMem.val_nat (now_serving + n)))
+                **
+                (monoBlack 0 ge_PreOrder now_serving)
+                **
+                (monoBlack 1 (@partial_map_PreOrder nat nat) f)
+                **
+                (⌜forall m (LT: now_serving + n < m), f m = None⌝)
+                **
+                (monoWhite 1 (@partial_map_PreOrder nat nat) (partial_map_singleton now_serving i))
+                **
+                (Eventually i (points_to TicketLock.now_serving (SCMem.val_nat now_serving)))
+                **
+                (waiters now_serving n))
+  .
+
+  Lemma sim: ModSim.mod_sim TicketLock.mod FairLock.mod.
+  Proof.
+    refine (@ModSim.mk _ _ (mk_wf Ord.lt_well_founded) nat_wf _ _ Σ _ _ _).
+    { econs. exact 0. }
+    { i. exists (S o0). ss. }
+    { admit. }
+    { cut ((forall tid,
+               (I ⊢ fsim I tid itop6 itop6 (fun r_src r_tgt os => I ** ⌜r_src = r_tgt /\ os = []⌝) (FairLock.lock_fun tt) (OMod.close_itree TicketLock.omod (SCMem.mod [1; 1]) (TicketLock.lock_fun tt)) [])) /\
+             (forall tid,
+                 (I ⊢ fsim I tid itop6 itop6 (fun r_src r_tgt os => I ** ⌜r_src = r_tgt /\ os = []⌝) (FairLock.unlock_fun tt) (OMod.close_itree TicketLock.omod (SCMem.mod [1; 1]) (TicketLock.unlock_fun tt)) []))).
+      { admit. }
+      split.
+      { i. iIntros "INV". unfold FairLock.lock_fun, TicketLock.lock_fun.
+        rred. rred. rewrite close_itree_call. ss. rred.
+        iApply (@fsim_sync _ _ _ _ _ _ _ None). ss. iFrame. iIntros "INV _".
+        rred. unfold SCMem.cas_fun, Mod.wrap_fun. rred.
+        iDestruct "INV" as "[[%m [MEM ST]] [%w [MONO H]]]".
+        iApply fsim_getR. iSplit.
+        { iFrame. }
+        rred. iApply fsim_tauR. rred.
+
+        unfold SCMem.cas.
+        destruct w; ss.
+        { iDestruct "H" as "[[POINTL POINTF] EXCL]".
+          iPoseProof (memory_ra_load with "MEM POINTL") as "%". ss. des; clarify.
+          rewrite H. ss.
+          iPoseProof (memory_ra_store with "MEM POINTL") as "[% [% > [MEM POINTL]]]".
+          rewrite H1. ss.
+          rred. iApply fsim_getR. iSplit.
+          { iFrame. }
+          rred. iApply (fsim_putR with "ST"). iIntros "ST".
+          rred. iApply fsim_tauR.
+          rred. iApply fsim_tauR.
+
+          iApply (@fsim_alloc_obligation _ _ _ _ _ _ _ (Ord.large × 10)%ord). iIntros "% ONG NEG # POS".
+          iDestruct (monoBlack_alloc le_PreOrder 0) as "-# > [% ORD]".
+          iPoseProof (black_updatable with "MONO") as "> MONO".
+          { instantiate (1:=W_own k k0). econs. }
+          iPoseProof (black_persistent_white with "MONO") as "# MWHITE".
+          iPoseProof (Neg_split with "NEG") as "> [FUEL NEG]". { eapply ord_mult_split. }
+          rred. iApply (@fsim_yieldR _ _ _ _ _ _ _ None). iSplitR "EXCL NEG".
+          { ss. iFrame. iSplit; auto. iSplitL "MEM ST".
+            { iExists _. iFrame. }
+            iExists _. iFrame. iSplit.
+            { iExists _. iFrame. auto. }
+            { iClear "POINTF ORD". iModIntro. iExists _. eauto. }
+          }
+          iIntros "INV _".
+          iPoseProof (Neg_split with "NEG") as "> [FUEL NEG]". { eapply ord_mult_split. }
+          rred. iApply fsim_tauR.
+          rred. iApply (@fsim_yieldR _ _ _ _ _ _ _ None). ss. iFrame.
+          iIntros "INV _".
+          iPoseProof (Neg_split with "NEG") as "> [FUEL NEG]". { eapply ord_mult_split. }
+
+        rred. iApply fsim_tauR.
+        rred. rewrite close_itree_call. ss.
+        rred. iApply (@fsim_yieldR _ _ _ _ _ _ _ None). ss. iFrame.
+        iIntros "INV _".
+        iPoseProof (Neg_split with "NEG") as "> [FUEL NEG]". { eapply ord_mult_split. }
+
+        unfold SCMem.store_fun, Mod.wrap_fun.
+        iDestruct "INV" as "[[% [MEM ST]] [% [MONO H]]]".
+        rred. iApply fsim_getR. iSplit.
+        { iFrame. }
+        rred. iApply fsim_tauR. rred.
+
+        iPoseProof (black_white_compare with "MWHITE MONO") as "%". inv H2.
+        ss. iDestruct "H" as "[[POINTL [% [[POINTF ORD] %]]] EVT]".
+
+        iPoseProof (memory_ra_store with "MEM POINTF") as "[% [% > [MEM POINTF]]]".
+        rewrite H3. ss.
+        rred. iApply fsim_getR. iSplit.
+        { iFrame. }
+        rred. iApply (fsim_putR with "ST"). iIntros "ST".
+        rred. iApply fsim_tauR.
+        rred. iApply fsim_tauR.
+        iPoseProof (eventually_finish with "EVT") as "[# DONE | [ONG EVT]]".
+        { iApply (fsim_obligation_not_done with "DONE"). ss. auto. }
+        iPoseProof (black_updatable with "ORD") as "> ORD".
+        { instantiate (1:=1). lia. }
+        iPoseProof (black_persistent_white with "ORD") as "#WHITE".
+        iApply (fsim_dealloc_obligation with "ONG").
+        { ss. }
+        iIntros "# DONE". iPoseProof ("EVT" with "DONE WHITE") as "EVT".
+
+        rred. iApply (@fsim_sync _ _ _ _ _ _ _ None). iSplitR "".
+        { ss. unfold I. iSplit; auto. iSplit; auto. iSplitL "MEM ST".
+          { iExists _. iFrame. }
+          iExists _. iFrame. ss. iFrame.
+          iExists _. iFrame. auto.
+        }
+        iIntros "INV _". iApply fsim_tauR. iApply fsim_ret. auto.
+      }
+
+      { iDestruct "H" as "[[POINTL POINTF] EXCL]".
+        iPoseProof (memory_ra_load with "MEM POINTL") as "%". des; clarify.
+        iPoseProof (eventually_obligation with "EXCL") as "# [% OBL]".
+        rewrite H. ss.
+        rred. iApply fsim_tauR.
+        rred.
+        iPoseProof (black_persistent_white with "MONO") as "# WHITE".
+        iAssert I with "[MEM ST MONO POINTL POINTF EXCL]" as "INV".
+        { unfold I. iSplitL "MEM ST".
+          { iExists _. iFrame. }
+          iExists (W_own _ _). ss. iFrame.
+        }
+        iStopProof.
+        pattern n. revert n. eapply (well_founded_induction Ord.lt_well_founded). intros o IH.
+        iIntros "[# [OBL WHITE] INV]".
+        rewrite unfold_iter_eq. rred.
+        iApply (@fsim_yieldR _ _ _ _ _ _ _ (Some k)).
+        ss. iFrame. iSplitL.
+        { iExists _. eauto. }
+        iIntros "INV FUEL".
+        rred. iApply fsim_tauR.
+        rred. rewrite close_itree_call. ss.
+        unfold SCMem.load_fun, Mod.wrap_fun. ss.
+        rred. iApply (@fsim_yieldR _ _ _ _ _ _ _ None). ss. iFrame. iIntros "INV _".
+        iDestruct "INV" as "[[% [MEM ST]] [% [MONO H]]]".
+        rred. iApply fsim_getR. iSplit. { iFrame. }
+        rred. iApply fsim_tauR. rred.
+        iPoseProof (black_white_compare with "WHITE MONO") as "%". inv H1.
+        ss. iDestruct "H" as "[[POINTL [% [[POINTF PWHITE] %]]] EVT]".
+        iPoseProof (memory_ra_load with "MEM POINTF") as "%".
+        destruct H2 as [LOAD _]. rewrite LOAD.
+        rred. iApply fsim_tauR.
+        rred. des; subst; cycle 1.
+        { iApply (@fsim_yieldR _ _ _ _ _ _ _ None). ss. iSplitL.
+          { iSplit; auto. iSplit; auto. unfold I. iSplitL "MEM ST".
+            { iExists _. iFrame. }
+            iExists (W_own _ _). ss. iFrame. iExists _. iFrame. auto.
+          }
+          iIntros "INV _".
+          rred. iApply fsim_tauR.
+          rred. rewrite close_itree_call. ss.
+          unfold SCMem.compare_fun, Mod.wrap_fun.
+          rred. iApply (@fsim_yieldR _ _ _ _ _ _ _ None). ss. iFrame. iIntros "INV _".
+          iDestruct "INV" as "[[% [MEM ST]] [% [MONO H]]]".
+          rred. iApply fsim_getR. iSplit; [eauto|].
+          rred. iApply fsim_tauR.
+          rred. iApply fsim_tauR.
+          rred. iApply (@fsim_sync _ _ _ _ _ _ _ None). ss. iSplitL.
+          { iSplit; auto. iSplit; auto. unfold I. iSplitL "MEM ST".
+            { iExists _. iFrame. }
+            { iExists _. iFrame. }
+          }
+          iIntros "INV _". rred. iApply fsim_tauR.
+          rred. iApply fsim_ret. auto.
+        }
+        { iDestruct "FUEL" as "[FUEL|#DONE]"; cycle 1.
+          { iDestruct (eventually_done with "DONE EVT") as "[H EVT]".
+            iPoseProof (black_white_compare with "H PWHITE") as "%". exfalso. lia.
+          }
+          rred. iApply (@fsim_yieldR _ _ _ _ _ _ _ None). ss. iSplitR "FUEL".
+          { iSplit; auto. iSplit; auto. unfold I. iSplitL "MEM ST".
+            { iExists _. iFrame. }
+            { iExists _. iFrame. unfold I_aux. iFrame. iExists _. iFrame. auto. }
+          }
+          iIntros "INV _".
+          rred. iApply fsim_tauR.
+          rred. rewrite close_itree_call. ss.
+          unfold SCMem.compare_fun, Mod.wrap_fun. ss.
+          rred. iApply (@fsim_yieldR _ _ _ _ _ _ _ None). ss. iFrame. iIntros "INV _".
+          rred. iDestruct "INV" as "[[% [MEM ST]] [% [MONO H]]]".
+          iApply fsim_getR. iSplit. { iFrame. }
+          rred. iApply fsim_tauR.
+          rred. iApply fsim_tauR.
+          rred. iApply (@fsim_yieldR _ _ _ _ _ _ _ None). ss. iSplitR "FUEL".
+          { iSplit; auto. iSplit; auto. unfold I. iSplitL "MEM ST".
+            { iExists _. iFrame. }
+            { iExists _. iFrame. }
+          }
+          iIntros "INV _".
+          rred. iApply fsim_tauR.
+          rred. iApply fsim_tauR.
+          iPoseProof (Pos_Neg_annihilate with "OBL FUEL") as "> [% [H %]]".
+          iClear "OBL". iPoseProof (Pos_persistent with "H") as "# OBL".
+          iApply IH; eauto. iSplit; auto. iClear "INV H". auto.
+        }
+      }
+    }
+  Admitted.
+End SIM.
