src/Wrapper.v
@@ -1,0 +1,90 @@
+From sflib Require Import sflib.
+From Paco Require Import paco.
+Require Import Coq.Classes.RelationClasses Lia Program.
+From Fairness Require Export ITreeLib WFLib FairBeh NatStructs Mod pind OpenMod.
+
+Set Implicit Arguments.
+
+
+Module WMod.
+  Variant output (state: Type) (ident: ID) (mident: ID) (R: Type) :=
+    | normal (st: state) (r: R) (fm: fmap (id_sum ident mident))
+    | stuck
+    | disabled
+  .
+
+  Record function (state: Type) (ident: ID) (mident: ID): Type :=
+    mk_fun {
+        type: ident;
+        A: Type;
+        R: Type;
+        body: thread_id -> A -> state -> output state ident mident R -> Prop;
+      }.
+
+  Record t: Type :=
+    mk {
+        state: Type;
+        ident: ID;
+        mident: ID;
+        st_init: state;
+        funs: list (fname * function state ident mident);
+      }.
+
+  Section INTERP.
+    Variable m: t.
+
+    Definition interp_state := (m.(state) * NatMap.t m.(ident))%type.
+
+    Definition interp_ident := id_sum thread_id m.(mident).
+
+    Definition interp_fmap
+               (fm: fmap (id_sum m.(ident) m.(mident))) (ts: NatMap.t m.(ident)) : fmap interp_ident :=
+      fun i =>
+        match i with
+        | inl i =>
+            match NatMap.find i ts with
+            | Some i => fm (inl i)
+            | None => Flag.emp
+            end
+        | inr i => fm (inr i)
+        end.
+
+    Definition interp_fun (f: function m.(state) m.(ident) m.(mident))
+      : ktree (((@eventE interp_ident) +' cE) +' sE interp_state) Any.t Any.t :=
+      Mod.wrap_fun
+        (fun (arg: f.(A)) =>
+           _ <- trigger Yield;;
+
+           tid <- trigger (GetTid);;
+           '(st, ts) <- trigger (@Get _);;
+           let ts := NatMap.add tid f.(type) ts in
+           _ <- trigger (Put (st, ts));;
+
+           ITree.iter
+             (fun (_: unit) =>
+                b <- trigger (Choose bool);;
+                if (b: bool) then _ <- trigger Yield;; Ret (inl tt)
+                else
+                  '(st, ts) <- trigger (@Get _);;
+                  next <- trigger (Choose (sig (f.(body) tid arg st)));;
+                  match proj1_sig next with
+                  | normal st r fm =>
+                      let ts := NatMap.remove tid ts in
+                      _ <- trigger (Fair (interp_fmap fm ts));;
+                      _ <- trigger (Put (st, ts));;
+                      _ <- trigger Yield;;
+                      Ret (inr r)
+                  | stuck _ _ _ _ => UB
+                  | disabled _ _ _ _ => _ <- trigger Yield;; Ret (inl tt)
+                  end) tt)
+    .
+
+    Definition interp_mod: Mod.t :=
+      Mod.mk
+        (m.(st_init), NatMap.empty m.(ident))
+        (Mod.get_funs (List.map (fun '(fn, f) => (fn, interp_fun f)) m.(funs)))
+    .
+  End INTERP.
+End WMod.
+Arguments WMod.disabled {_ _ _ _}.
+Arguments WMod.stuck {_ _ _ _}.
